Module structure reorg (#71)
Reorg

<small>By submitting this pull request, I confirm that my contribution
is made under the terms of the [MIT
license](https://github.com/dafny-lang/dafny/blob/master/LICENSE.txt).</small>

---------

Co-authored-by: John Tristan <trjohnb@amazon.com>

src/interop/cs/DRandomCoin.cs
@@ -6,7 +6,7 @@
 using System;
 using System.Numerics;
 
-namespace BaseInterface {
+namespace CoinInterface {
 
     public class DRandomCoin {
 
