src/Distributions/Bernoulli/Model.dfy
@@ -3,21 +3,21 @@
  *  SPDX-License-Identifier: MIT
  *******************************************************************************/
 
-include "../Uniform/Model.dfy"
+include "../Uniform/Uniform.dfy"
 include "../../ProbabilisticProgramming/Monad.dfy"
 
 module BernoulliModel {
-  import UniformModel
+  import Uniform
   import Monad
 
   // Footnote 5, p. 82
-  function ProbBernoulli(numer: nat, denom: nat): (f: Monad.Hurd<bool>)
+  function Sample(numer: nat, denom: nat): (f: Monad.Hurd<bool>)
     requires denom != 0
     requires numer <= denom
-    ensures forall s :: f(s).0 == (UniformModel.ProbUniform(denom)(s).0 < numer)
-    ensures forall s :: f(s).1 == UniformModel.ProbUniform(denom)(s).1
+    ensures forall s :: f(s).0 == (Uniform.Model.Sample(denom)(s).0 < numer)
+    ensures forall s :: f(s).1 == Uniform.Model.Sample(denom)(s).1
   {
-    Monad.Bind(UniformModel.ProbUniform(denom), (k: nat) => Monad.Return(k < numer))
+    Monad.Bind(Uniform.Model.Sample(denom), (k: nat) => Monad.Return(k < numer))
   }
 
 }
