src/Distributions/Bernoulli/Bernoulli.dfy
@@ -1,0 +1,11 @@
+include "Correctness.dfy"
+include "Implementation.dfy"
+include "Interface.dfy"
+include "Model.dfy"
+
+module Bernoulli {
+  import Interface = BernoulliInterface
+  import Implementation = BernoulliImplementation
+  import Correctness = BernoulliCorrectness
+  import Model = BernoulliModel
+}
