src/Distributions/Coin/Coin.dfy
@@ -1,0 +1,7 @@
+include "Interface.dfy"
+include "Model.dfy"
+
+module Coin {
+  import Interface = CoinInterface
+  import Model = CoinModel
+}
