src/Distributions/Uniform/Uniform.dfy
@@ -1,0 +1,11 @@
+include "Correctness.dfy"
+include "Implementation.dfy"
+include "Interface.dfy"
+include "Model.dfy"
+
+module Uniform {
+  import Interface = UniformInterface
+  import Implementation = UniformImplementation
+  import Correctness = UniformCorrectness
+  import Model = UniformModel
+}
