src/Distributions/UniformPowerOfTwo/UniformPowerOfTwo.dfy
@@ -1,0 +1,11 @@
+include "Correctness.dfy"
+include "Implementation.dfy"
+include "Interface.dfy"
+include "Model.dfy"
+
+module UniformPowerOfTwo {
+  import Interface = UniformPowerOfTwoInterface
+  import Implementation = UniformPowerOfTwoImplementation
+  import Correctness = UniformPowerOfTwoCorrectness
+  import Model = UniformPowerOfTwoModel
+}
